experiment: 3-way memory everywhere, i.e. "map word (option byte)", where "Some None" means "reserved for MMIO or other special things"

src/MinimalMMIO.v
@@ -15,23 +15,34 @@ Require Export riscv.MMIOTrace.
 Require Export riscv.RiscvMachine.
 Require Import Coq.micromega.Lia.
 Require Import coqutil.Map.Interface.
+Require Import coqutil.Datatypes.HList.
 Require Import coqutil.Tactics.Tactics.
 
 
 Local Open Scope Z_scope.
 Local Open Scope bool_scope.
 
+Definition all_None{A: Type}{n: nat}(t: tuple (option A) n): bool :=
+  List.fold_right (fun o b => match o with
+                              | Some _ => false
+                              | None => true
+                              end)
+                  true
+                  (tuple.to_list t).
+
 Section Riscv.
 
   Context {W: Words}.
-  Context {Mem: map.map word byte}.
+  Context {Mem: map.map word (option byte)}.
   Context {RFF: RegisterFileFunctions Register word}.
 
   Local Notation RiscvMachineL := (RiscvMachine Register MMIOAction).
 
-  Definition theMMIOAddr: word := (ZToReg 65524). (* maybe like spike *)
-
-  Definition simple_isMMIOAddr: word -> bool := reg_eqb theMMIOAddr.
+  Definition isMMIOAddr(sz: nat)(a: word)(m: Mem): bool :=
+    match map.getmany_of_tuple m (Memory.footprint a sz) with
+    | Some optbytes => all_None optbytes
+    | None => false
+    end.
 
   Definition logEvent(e: LogItem MMIOAction): OStateND RiscvMachineL unit :=
     m <- get; put (withLogItem e m).
@@ -84,25 +95,14 @@ Section Riscv.
         mach <- get;
         match Memory.loadWord mach.(getMem) a with
         | Some v => Return v
-        | None => if simple_isMMIOAddr a then
+        | None => if isMMIOAddr 4 a mach.(getMem) then
                     inp <- arbitrary w32;
                     logEvent ((mach.(getMem), MMInput, [a]), (mach.(getMem), [uInt32ToReg inp]));;
                     Return inp
                   else
-                    fail_hard
+                     fail_hard
         end;
       loadDouble := loadN 8;
-(*
-      storeWord a v :=
-        mach <- get;
-        if mach.(isMem) a then
-          liftStore Memory.storeWord a v
-        else
-          if simple_isMMIOAddr a then
-            logEvent (MMOutput, [a; uInt32ToReg v], [])
-          else
-            fail_hard;
-*)
 
       storeByte   := storeN 1;
       storeHalf   := storeN 2;
@@ -110,7 +110,7 @@ Section Riscv.
         mach <- get;
         match Memory.storeWord mach.(getMem) a v with
         | Some m => put (withMem m mach)
-        | None => if simple_isMMIOAddr a then
+        | None => if isMMIOAddr 4 a mach.(getMem) then
                     logEvent ((mach.(getMem), MMOutput, [a; uInt32ToReg v]), (mach.(getMem), []))
                   else
                     fail_hard
@@ -161,7 +161,7 @@ Section Riscv.
                             get, put, fail_hard,
                             arbitrary,
                             logEvent,
-                            simple_isMMIOAddr, theMMIOAddr,
+                            all_None, List.fold_right, tuple.to_list,
                             ZToReg, MkMachineWidth.MachineWidth_XLEN,
                             fail_if_None, loadN, storeN in *;
                      subst;
@@ -226,12 +226,12 @@ Section Riscv.
   Instance MinimalMMIOSatisfiesPrimitives: Primitives MMIOAction (OStateND RiscvMachineL) := {|
     Primitives.mcomp_sat := @OStateNDOperations.computation_with_answer_satisfies RiscvMachineL;
     Primitives.nonmem_loadWord_sat initialL addr post :=
-      simple_isMMIOAddr addr = true /\
+      isMMIOAddr 4 addr initialL.(getMem) = true /\
       forall v, post v (withLogItem ((initialL.(getMem), MMInput, [addr]),
                                      (initialL.(getMem), [word.of_Z (LittleEndian.combine 4 v)]))
                                     initialL);
     Primitives.nonmem_storeWord_sat initialL addr v post :=
-      simple_isMMIOAddr addr = true /\
+      isMMIOAddr 4 addr initialL.(getMem) = true /\
       post (withLogItem
               ((initialL.(getMem), MMOutput, [addr; word.of_Z (LittleEndian.combine 4 v)]),
                (initialL.(getMem), []))
@@ -264,7 +264,7 @@ Section Riscv.
           reflexivity.
         * t.
       + right.
-        destruct (simple_isMMIOAddr addr) eqn: G.
+        destruct (isMMIOAddr 4 addr (getMem initialL)) eqn: G.
         * t.
           match goal with
           | |- post ?inp ?mach => specialize (H (Some (inp, mach)))
@@ -272,7 +272,6 @@ Section Riscv.
           destruct H; [|t].
           (* hypothesis of H *) right. do 2 eexists; split; [reflexivity|]. t.
         * exfalso.
-          t.
           specialize (H None).
           destruct H; [|t].
           right.
@@ -288,17 +287,13 @@ Section Riscv.
         end.
         destruct H; [|solve [t]].
         t.
-        * right.
-          do 2 eexists; split; [reflexivity|]. simpl.
-          rewrite F.
-          reflexivity.
-        * right.
+        right.
           do 2 eexists; split; [reflexivity|]. simpl.
           rewrite F.
           reflexivity.
       + destruct (Memory.loadWord (getMem initialL) addr) eqn: G; [ exfalso; t | ].
         right.
-        destruct (simple_isMMIOAddr addr) eqn: A.
+        destruct (isMMIOAddr 4 addr (getMem initialL)) eqn: A.
         * t.
           match goal with
           | |- post ?inp ?mach => specialize (H (Some (inp, mach)))
@@ -306,7 +301,6 @@ Section Riscv.
           destruct H; [|t].
           (* hypothesis of H *) right. do 2 eexists; split; [reflexivity|]. t.
         * exfalso.
-          t.
           specialize (H None).
           destruct H; [|t].
           right.
@@ -334,8 +328,9 @@ Section Riscv.
   Instance MinimalMMIOSatisfiesMMIOAxioms:
     AxiomaticRiscvMMIO (OStateND RiscvMachineL).
   Proof.
-    constructor. all: t.
-  Qed.
+    constructor.
+    all: t.
+  Admitted. (* TODO! *)
 
 End Riscv.
 
